Some improvements and small unit tests

iocy/FancyTraces2.fsti
@@ -1,7 +1,14 @@
 module FancyTraces2
 
 open FStar.Tactics
+
 open FStar.List.Tot
+
+(**
+val rev_append: l1:list 'a -> l2:list 'a ->
+  Lemma (requires True)
+        (ensures ((rev (l1@l2)) == ((rev l2)@(rev l1))))
+  [SMTPat (rev (l1@l2))]**)
 
 val promise (e:Type u#a) (a:Type u#b) : Type u#(max a b)
 
@@ -27,7 +34,6 @@ val mem (pr:promise 'e 'a) (pts:parallel_traces 'e) : Type0
 val sel_lt (pr:promise 'e 'a) (pts:(parallel_traces 'e){pr `mem` pts}) : atrace 'e
 val sel_r (pr:promise 'e 'a) (pts:(parallel_traces 'e){pr `mem` pts}) : 'a
 
-
 let ord #e (pts pts':parallel_traces e) =
   (forall a (x:promise e a). x `mem` pts ==> x `mem` pts') /\
   (forall a (x:promise e a). x `mem` pts ==> (sel_lt x pts' `suffix_of` sel_lt x pts))
@@ -36,13 +42,26 @@ let ord_reflexive #e (pts:parallel_traces e) : Lemma (ord pts pts) = ()
 let ord_transitive #e (pts pts' pts'':parallel_traces e) :
   Lemma (ord pts pts' /\ ord pts' pts'' ==> ord pts pts'') = ()
 
-val insert (r:'a) (lt:atrace 'e) (pts:parallel_traces 'e) :
-  pr:(promise 'e 'a){~(pr `mem` pts)}
-  &
-  pts':(parallel_traces 'e){pts `ord` pts'} // /\ pr `mem` pts' /\ sel pr pts' == lt}
+val async (r:'a) (lt:atrace 'e) (pts:parallel_traces 'e) :
+  prpts':((promise 'e 'a) & (parallel_traces 'e)){
+    ~(fst prpts' `mem` pts) /\ pts `ord` (snd prpts') /\
+    fst prpts' `mem` snd prpts' /\ sel_r (fst prpts') (snd prpts') == r /\ sel_lt (fst prpts') (snd prpts') == lt}
 
-val await_pr (pr:promise 'e 'a) (pts:(parallel_traces 'e){pr `mem` pts}) :
-  pts':(parallel_traces 'e){pts `ord` pts'}
+(**
+val lemma_async (r:'a) (lt:atrace 'e) (pts:parallel_traces 'e) :
+  Lemma (
+    let prpts' = async r lt pts in
+    ~(fst prpts' `mem` pts) /\ pts `ord` (snd prpts') /\
+    fst prpts' `mem` snd prpts' /\ sel_r (fst prpts') (snd prpts') == r /\ sel_lt (fst prpts') (snd prpts') == lt)
+  [SMTPat (fst (async r lt pts) `mem` pts);
+   SMTPat (pts `ord` (snd (async r lt pts)));
+   SMTPat (fst (async r lt pts) `mem` snd (async r lt pts));
+   SMTPat (sel_r (fst (async r lt pts)) (snd (async r lt pts)));
+   SMTPat (sel_lt (fst (async r lt pts)) (snd (async r lt pts)))]
+**)
+
+val await (pr:promise 'e 'a) (pts:(parallel_traces 'e){pr `mem` pts}) :
+  pts':(parallel_traces 'e){pts `ord` pts' /\ sel_lt pr pts' == []}
 
 // val size : atrace 'e -> nat
 
@@ -62,22 +81,41 @@ val closed_atrace (pts:parallel_traces 'e) (tr:atrace 'e) : GTot Type0 //(decrea
   //   closed_atrace (dsnd (insert pr lt m)) (lt@tl) (** the parent thread can await on the promise of the kid
   //                                              and promises returned/created by the kid *)
 
-val closed_atrace_insert #e #a h (pts:parallel_traces e) (r:a) lt :
+val closed_atrace_async #e #a h (pts:parallel_traces e) (r:a) lt :
   Lemma
-    (requires (closed_atrace pts (h@lt)))
+    (requires (closed_atrace pts ((rev lt) @ h)))
     (ensures (
-      let (| pr, pts' |) = insert r lt pts in
-      closed_atrace pts' (h @ [EAsync pr r lt])))
+      let (pr, pts') = async r lt pts in
+      closed_atrace pts' ((EAsync pr r lt) :: h)))
+    [SMTPat (closed_atrace (snd (async r lt pts)) ((EAsync (fst (async r lt pts)) r lt) :: h))]
+//     SMTPat (closed_atrace (snd (async r lt pts)) ([EAsync (fst (async r lt pts)) r lt] @ h));
+//     SMTPat (closed_atrace (snd (async r lt pts)) ([EAsync (fst (async r lt pts)) r lt] @ h)) ]
 
 val closed_atrace_await_pr #e #a (pr:promise e a) h pts :
   Lemma
     (requires (closed_atrace pts h))
-    (ensures (closed_atrace (await_pr pr pts) (h @ [EAwait pr])))
+    (ensures (closed_atrace (await pr pts) ((EAwait pr) :: h)))
+    [SMTPat (closed_atrace (await pr pts) ((EAwait pr) :: h))]
 
 val closed_atrace_produce #e (ev:e) h pts :
   Lemma
     (requires (closed_atrace pts h))
-    (ensures (closed_atrace pts (h @ [Ev ev])))
+    (ensures (closed_atrace pts ((Ev ev) :: h)))
+    [SMTPat (closed_atrace pts ((Ev ev) :: h))]
+
+let closed_atrace_append_assoc #e h lt1 lt2 (pts:parallel_traces e) :
+  Lemma
+    (closed_atrace pts (lt1@(lt2@h)) <==>  closed_atrace pts ((lt1@lt2)@h))
+    [SMTPat (closed_atrace pts (lt1@(lt2@h)));
+     SMTPat (closed_atrace pts ((lt1@lt2)@h))]
+  = append_assoc lt1 lt2 h
+
+let closed_atrace_rev_append #e h lt1 lt2 (pts:parallel_traces e) :
+  Lemma
+    (closed_atrace pts ((rev (lt1@lt2))@h) <==>  closed_atrace pts ((rev lt2) @ (rev lt1) @ h))
+    [SMTPat (closed_atrace pts ((rev (lt1@lt2))@h));
+     SMTPat (closed_atrace pts ((rev lt2) @ (rev lt1)@h))]
+  = rev_append lt1 lt2
 
 // val interleave_map
 //   (pts: parallel_traces 'e)
@@ -93,73 +131,173 @@ let w_pre e = h:atrace e -> pts:parallel_traces e{
 let w_post e a h pts =
   a -> lt:atrace e -> pts':parallel_traces e{
       pts `ord` pts' /\
-      closed_atrace pts' (h @ lt)
+      closed_atrace pts' ((rev lt) @ h)
   } -> Type0
 
 let w e a = h:atrace e -> pts:parallel_traces e{closed_atrace pts h} -> w_post e a h pts -> Type0
 
+unfold
 let w_ord #e #a (w1 w2:w e a) =
   forall h pts post. w2 h pts post ==> w1 h pts post
 
+unfold
 let encode_pre_post_in_w #e #a
   (pre:w_pre e)
   (post:(h:atrace e -> pts:parallel_traces e -> w_post e a h pts))
   : w e a
   = (fun h pts p -> pre h pts /\ (forall r' lt' pts'. post h pts r' lt' pts' ==> p r' lt' pts'))
 
+unfold
 let w_return e #a (x:a) : w e a =
   fun h pts p -> p x [] pts
 
+unfold
 let w_bind #e #a #b (m:w e a) (f: a -> w e b) : w e b =
   fun h pts post ->
     m h pts (fun r' lt' pts' ->
-        f r' (h@lt') pts' (fun r'' lt'' pts'' ->
-        append_assoc h lt' lt'';
+        f r' ((rev lt')@h) pts' (fun r'' lt'' pts'' ->
         post r'' (lt'@lt'') pts''))
 
+unfold
 let w_async #e #a (wf:w e a) : w e (promise e a) =
   fun h pts post ->
+    (** CA: should wf get any pts' that extends pts? *)
     wf h pts (fun r' lt' pts' ->
-      let prpts'' = insert r' lt' pts' in
-      closed_atrace_insert h pts' r' lt';
-      post (dfst prpts'') [EAsync (dfst prpts'') r' lt'] (dsnd prpts''))
+      let prpts'' = async r' lt' pts' in
+      post (fst prpts'') [EAsync (fst prpts'') r' lt'] (snd prpts''))
 
+unfold
 let w_await #e #a (pr:promise e a) : w e a =
   fun h pts post ->
     pr `mem` pts /\
-    (closed_atrace_await_pr pr h pts;
-    post (sel_r pr pts) [EAwait pr] (await_pr pr pts))
+    post (sel_r pr pts) [EAwait pr] (await pr pts)
 
+unfold
 let w_produce #e (ev:e) : w e unit =
   fun h pts post ->
-    closed_atrace_produce ev h pts;
     post () [Ev ev] pts
 
-let (let!) = w_bind
+unfold
+let (let!) #e #a #b (m:w e a) (f: a -> w e b) : w e b = w_bind m f
 
+let _ =
+  assert (
+    (w_produce 0)
+    `w_ord`
+    encode_pre_post_in_w (fun _ _ -> True) (fun _ _ _ lt _ -> lt == [Ev 0]))
+
+let _ =
+  assert (
+    (w_produce 0 ;! w_produce 1 ;! w_produce 2)
+    `w_ord`
+    encode_pre_post_in_w (fun _ _ -> True) (fun _ _ _ lt _ -> lt == [Ev 0; Ev 1; Ev 2]))
+
+#push-options "--fuel 10"
+let _ =
+  assert (
+    (w_produce 0 ;! w_produce 1 ;! w_produce 2;! w_produce 2;! w_produce 2;! w_produce 2;! w_produce 2;! w_produce 2)
+    `w_ord`
+    encode_pre_post_in_w (fun _ _ -> True) (fun _ _ _ lt _ -> lt == [Ev 0; Ev 1; Ev 2; Ev 2; Ev 2; Ev 2; Ev 2; Ev 2]))
+#pop-options
+
+let test_await (pr:promise int unit) =
+  assert (
+    (w_await pr)
+    `w_ord`
+    encode_pre_post_in_w (fun _ pts -> pr `mem` pts) (fun _ _ _ lt _ -> lt == [EAwait pr]))
+
+let test_ev_await (pr:promise int unit) =
+  assert (
+    (w_await pr ;! w_produce 0)
+    `w_ord`
+    encode_pre_post_in_w (fun _ pts -> pr `mem` pts) (fun _ _ _ lt _ -> lt == [EAwait pr; Ev 0]))
+
+let test_async () =
+  assert (
+    (w_async (w_produce 5))
+    `w_ord`
+    encode_pre_post_in_w (fun _ _ -> True) (fun _ _ pr lt _ -> lt == [EAsync pr () [Ev 5]]))
+
+let test_async_ev () =
+  assert (
+    (let! _ = w_async (w_produce 5) in w_produce 2)
+    `w_ord`
+    encode_pre_post_in_w (fun _ _ -> True) (fun _ _ _ lt _ -> exists pr. lt == [EAsync pr () [Ev 5]; Ev 2]))
+
+let test_async_await () =
+  assert (
+    (let! pr = w_async (w_produce 5) in w_await pr)
+    `w_ord`
+    encode_pre_post_in_w (fun _ _ -> True) (fun _ _ _ lt _ -> exists pr. lt == [EAsync pr () [Ev 5]; EAwait pr]))
+
+let test_async_ev_await () =
+  assert (
+    (let! pr = w_async (w_produce 5) in w_produce 0 ;! w_await pr)
+    `w_ord`
+    encode_pre_post_in_w (fun _ _ -> True) (fun _ _ _ lt _ -> exists pr. lt == [EAsync pr () [Ev 5]; Ev 0; EAwait pr]))
+
+unfold
 let f (pr:promise int unit) : w int unit =
   w_await pr ;!
   w_produce 0
 
+unfold
 let g () : w int unit =
   let! pr'  = w_async (let! pr = w_async (w_produce (-2)) in f pr) in
   let! pr'' = w_async (w_produce (-1)) in
   w_await pr' ;!
   w_await pr''
 
+#push-options "--fuel 100 --z3rlimit 100"
 let _ =
   assert (
-    g ()
+    (let! pr = w_async (w_produce (-2)) in f pr)
     `w_ord`
-    encode_pre_post_in_w (fun _ _ -> True) (fun _ _ _ lt _ -> exists pr' lt' pr''. lt == [EAsync pr' () lt'; EAsync pr'' () [Ev (-1)]; EAwait pr'; EAwait pr''])
-  ) by (
-    norm [delta_only [`%encode_pre_post_in_w; `%w_ord;`%g];iota];
+    encode_pre_post_in_w (fun _ _ -> True) (fun _ _ _ lt _ ->
+      exists pr. lt == [EAsync pr () [Ev (-2)]; EAwait pr; Ev 0])
+  )
+
+let _ =
+  assert (
+    (w_async (let! pr = w_async (w_produce (-2)) in f pr))
+    `w_ord`
+    encode_pre_post_in_w (fun _ _ -> True) (fun _ _ pr' lt _ ->
+      exists pr. lt == [EAsync pr' () [EAsync pr () [Ev (-2)]; EAwait pr; Ev 0]])
+  )
+  by (
+    norm [delta_only [`%encode_pre_post_in_w; `%w_ord;`%g;`%f];iota];
+    norm [delta_only [`%w_async;`%w_produce;`%w_await;`%w_bind;`%op_let_Bang];iota];
     let h = forall_intro () in
     let pts = forall_intro () in
     let post = forall_intro () in
     let hyp = implies_intro () in
     let (_, hyp') = destruct_and hyp in
     clear hyp;
-    norm [delta_only [`%w_async;`%w_produce;`%w_await;`%w_bind];iota];
     simpl ();
+    FStar.Tactics.V1.Logic.split ();
+    bump_nth 2;
+    smt ();
+    smt ();
     dump "H")
+
+let _ =
+  assert (
+    g ()
+    `w_ord`
+    encode_pre_post_in_w (fun _ _ -> True) (fun _ _ _ lt _ ->
+      exists pr' pr pr''. lt == [EAsync pr' () [EAsync pr () [Ev (-2)]; EAwait pr; Ev 0]; EAsync pr'' () [Ev (-1)]; EAwait pr'; EAwait pr''])
+  )
+  by (
+    norm [delta_only [`%encode_pre_post_in_w; `%w_ord;`%g];iota];
+    norm [delta_only [`%w_async;`%w_produce;`%w_await;`%w_bind;`%op_let_Bang];iota];
+    let h = forall_intro () in
+    let pts = forall_intro () in
+    let post = forall_intro () in
+    let hyp = implies_intro () in
+    let (_, hyp') = destruct_and hyp in
+    clear hyp;
+    simpl ();
+    let hyp = instantiate hyp' (`()) in
+    clear hyp';
+    dump "H")
+#pop-options
